tests/lean/run/partial_fixpoint_coinductive_pred.lean
@@ -46,6 +46,7 @@ def infinite_chain {α} (step : α → Option α) (x : α) : Prop :=
   ∃ y, step x = some y ∧ (infinite_chain step y)
   partial_fixpoint
 
+
 theorem infinite_chain.intro {α} (step : α → Option α) (y x : α) :
     step x = some y → infinite_chain step y → infinite_chain step x := by
   intros; unfold infinite_chain; simp [*]
